Core/Term/BEq.lean
@@ -89,59 +89,59 @@ def Term.beq : Term -> Term -> Bool
 | tbind A1 K1 t1, tbind A2 K2 t2 => A1 == A2 && K1 == K2 && beq t1 t2
 | lam A1 t1, lam A2 t2 => A1 == A2 && beq t1 t2
 | guard a1 b1 c1, guard a2 b2 c2 => beq a1 a2 && beq b1 b2 && beq c1 c2
-| .match n1 a1 b1 c1 d1, .match n2 a2 b2 c2 d2 =>
-  if h : n1 = n2 then
-    let c : Vect n1 Bool := λ i => beq (c1 i) (c2 (by rw [h] at i; exact i))
-    let p : Vect n1 Bool := λ i => beq (b1 i) (b2 (by rw[h] at i; exact i))
-    beq a1 a2 && Vect.fold true (·&&·) c && Vect.fold true (·&&·) p && beq d1 d2
-  else false
+| .mtch n1 a1 b1 c1 d1, .mtch n2 a2 b2 c2 d2 => true -- TODO: Fix
+  -- if h : n1 = n2 then
+  --   let c : Vect n1 Bool := λ i => beq (c1 i) (c2 (by rw [h] at i; exact i))
+  --   let p : Vect n1 Bool := λ i => beq (b1 i) (b2 (by rw[h] at i; exact i))
+  --   beq a1 a2 && Vect.fold true (·&&·) c && Vect.fold true (·&&·) p && beq d1 d2
+  -- else false
 | _, _ => false
 
 instance instBEq_Term : BEq Term where
   beq := Term.beq
 
 instance instReflBEq_Term : ReflBEq Term where
-  rfl := by
-    intro a; induction a <;> simp [instBEq_Term, Term.beq] at *
-    all_goals (repeat assumption)
-    constructor; assumption; assumption
-    constructor; constructor; assumption; assumption; assumption
-    case «match» ih1 ih2 ih3 ih4 =>
-    constructor
-    · constructor
-      · constructor; assumption;
-        unfold Vect.fold;
-        case _ n _ _ _ _ =>
-        induction n
-        case _ => simp
-        case _ n ih v1 v2 =>
+  rfl := by sorry
+    -- intro a; induction a <;> simp [instBEq_Term, Term.beq] at *
+    -- all_goals (repeat assumption)
+    -- constructor; assumption; assumption
+    -- constructor; constructor; assumption; assumption; assumption
+    -- case «match» ih1 ih2 ih3 ih4 =>
+    -- constructor
+    -- · constructor
+    --   · constructor; assumption;
+    --     unfold Vect.fold;
+    --     case _ n _ _ _ _ =>
+    --     induction n
+    --     case _ => simp
+    --     case _ n ih v1 v2 =>
 
-          -- split
-          -- simp;
-        -- case _ => rfl
-        -- case _ =>
-        --   split; case _ h =>
-        --   cases h; simp at *
-        --   constructor
-        --   apply ih3
-          sorry
-      · sorry
-    · assumption
+    --       -- split
+    --       -- simp;
+    --     -- case _ => rfl
+    --     -- case _ =>
+    --     --   split; case _ h =>
+    --     --   cases h; simp at *
+    --     --   constructor
+    --     --   apply ih3
+    --       sorry
+    --   · sorry
+    -- · assumption
 
 instance instLawfulBEq_Term : LawfulBEq Term where
-  eq_of_beq := by
-    intro a b; cases a <;> simp [instBEq_Term] at *
-    all_goals (induction b <;>
-      simp [instBEq_Ctor0Variant, instBEq_Ctor1Variant, instBEq_Ctor2Variant, Term.beq] at *)
-    case _ => intro e; apply eq_of_beq e
-    case _ =>
-      intro e1 e2;
-      constructor
-      apply eq_of_beq e1
-      sorry
-    sorry
-    sorry
-    sorry
-    sorry
-    sorry
+  eq_of_beq := by sorry
+    -- intro a b; cases a <;> simp [instBEq_Term] at *
+    -- all_goals (induction b <;>
+    --   simp [instBEq_Ctor0Variant, instBEq_Ctor1Variant, instBEq_Ctor2Variant, Term.beq] at *)
+    -- case _ => intro e; apply eq_of_beq e
+    -- case _ =>
+    --   intro e1 e2;
+    --   constructor
+    --   apply eq_of_beq e1
+    --   sorry
+    -- sorry
+    -- sorry
+    -- sorry
+    -- sorry
+    -- sorry
 end Core
