README.md
@@ -1,6 +1,76 @@
 
 # System FD
 
+# Plan:
+
+## Closed Datatypes
+
+Generalize to multimatches with proper binders:
+(Allow wildcard patterns?)
+
+```
+match a, b with
+| Just x, Just y => t1
+| Just x, Nothing => t2
+| Nothing, _ => t3
+```
+
+The first pattern is of type `Vec n (Vec m (String x Nat) x Term)`
+(we don't need an inner `Vec`, but the scrutinees will force a Vec, so why not reuse the `m`)
+
+To determine if the match is exhaustive and unique, we can build an `m`-cube:
+Every case marks the relative part of the `m`-cube that has been tracked
+If at any point a position is double-marked then it is not unique
+If at any point a position is not marked then the match is not exhaustive
+
+reduction is via proper lifts, so a constructor `branch left right`
+is equivalent to `branch 2` and when the case is taken:
+
+```
+match (branch t1 t2) with
+| leaf 0 => c1
+| branch 2 => c2
+```
+
+then this reduces to `c1[σ]` where `σ = su t1 :: su t2 :: +0`
+(or rather `σ = [su t1, su t2] ++ +0`)
+i.e., a generalized beta substitution
+
+## Open Datatypes
+
+!!Guard is removed!!
+
+instances for open methods are treated as pattern match cases (just like closed data types)
+
+open methods are fully applied always? (I think yes, treat them like a match expression)
+
+if a match is exhaustive and unique, then you can't produce a + or a 0
+
+## Termination Predicate
+
+Add a parameter to the typing/globalwf judgement that characterizes a termination condition
+
+Later on we can pick one and show erasure relative to that
+
+
+
+
+
+
+
+
+
+
+
+
+
+
+
+
+
+
+
+
 The project is divided into 2 main directories
 
 ### SystemFD
